priqueue!

vfa/Binom.v
@@ -25,6 +25,8 @@ From Stdlib Require Import Strings.String. (* for manual grading *)
 From VFA Require Import Perm.
 From VFA Require Import Priqueue.
 
+From Stdlib Require Import FunctionalExtensionality.
+
 Module BinomQueue <: PRIQUEUE.
 
 Definition key := nat.
@@ -169,6 +171,20 @@ Fixpoint priq'  (i: nat) (l: list tree) : Prop :=
 
 Definition priq (q: priqueue) : Prop := priq' 0 q.
 
+(* priq has no restrictions on the length of q with same contents
+   this is a problem when prove the algorithm efficiency:
+   it is imposible to prove theorems like a well formed binom queue has length
+   O(log_2 n) *)
+Example x_priq_leading_leaf : forall n q, priq' n q -> priq' n (q ++ [Leaf]).
+Proof.
+  intros.
+  generalize dependent n.
+  induction q; intros; simpl.
+  - auto.
+  - simpl in H. destruct H as [? ?].
+    auto.
+Qed.
+
 (* ################################################################# *)
 (** * Proof of Algorithm Correctness *)
 
@@ -180,32 +196,94 @@ Definition priq (q: priqueue) : Prop := priq' 0 q.
 
 (** **** Exercise: 1 star, standard (empty_priq)  *)
 Theorem empty_priq: priq empty.
-(* FILL IN HERE *) Admitted.
+Proof.
+  unfold priq.
+  simpl. auto.
+Qed.
 (** [] *)
 
 (** **** Exercise: 2 stars, standard (smash_valid) *)
 Theorem smash_valid:
        forall n t u, pow2heap n t -> pow2heap n u -> pow2heap (S n) (smash t u).
-(* FILL IN HERE *) Admitted.
+Proof.
+  intros.
+  unfold smash.
+  destruct t; [| inv H].
+  destruct t2; auto.
+  destruct u; [| inv H0].
+  destruct u2; auto.
+  simpl in *.
+  bdestruct (k >? k0); simpl; split; auto; lia.
+Qed.
 (** [] *)
 
 (** **** Exercise: 3 stars, standard (carry_valid) *)
 Theorem carry_valid:
            forall n q,  priq' n q ->
            forall t, (t=Leaf \/ pow2heap n t) -> priq' n (carry q t).
-(* FILL IN HERE *) Admitted.
+Proof.
+  intros n q.
+  generalize dependent n.
+  induction q; intros.
+  - simpl. destruct t.
+    + unfold priq'. auto.
+    + auto.
+  - simpl. destruct a.
+    + destruct t; auto.
+      destruct H0; [inv H0|].
+      split; auto.
+      destruct H. destruct H; [inv H|].
+      apply IHq; [exact H1|].
+      right.
+      apply smash_valid; auto.
+    + simpl. split; auto. simpl in H. destruct H as [_ H]. auto.
+Qed.
 (** [] *)
 
 (** **** Exercise: 2 stars, standard, optional (insert_valid) *)
 Theorem insert_priq: forall x q, priq q -> priq (insert x q).
-(* FILL IN HERE *) Admitted.
+Proof.
+  unfold priq.
+  intros.
+  apply carry_valid; auto.
+  right. simpl. constructor.
+Qed.
 (** [] *)
 
 (** **** Exercise: 3 stars, standard, optional (join_valid) *)
 (* This proof is rather long, but each step is reasonably straightforward.
     There's just one [induction] to do, right at the beginning. *)
 Theorem join_valid: forall p q c n, priq' n p -> priq' n q -> (c=Leaf \/ pow2heap n c) -> priq' n (join p q c).
-(* FILL IN HERE *) Admitted.
+Proof.
+  induction p; intros.
+  - simpl. apply carry_valid; auto.
+  - simpl. destruct H.
+    destruct a, q.
+    + destruct c.
+      * split; auto. apply carry_valid; auto. right.
+        destruct H; [inv H|].
+        destruct H1; [inv H1|].
+        apply smash_valid; auto.
+      * split; auto.
+    + destruct t; destruct H0.
+      * split; auto. apply IHp; auto. right.
+        destruct H; [inv H|].
+        destruct H0; [inv H0|].
+        apply smash_valid; auto.
+      * destruct c; split; auto.
+        destruct H; [inv H|].
+        destruct H1; [inv H1|].
+        apply IHp; auto. right.
+        apply smash_valid; auto.
+    + simpl. split; auto.
+    + destruct t; destruct H0.
+      * destruct c; split; auto.
+        destruct H0; [inv H0|]. destruct H1; [inv H1|].
+        apply IHp; auto. right.
+        apply smash_valid; auto.
+      * split; auto.
+Qed.
+
 (** [] *)
 
 Theorem merge_priq:  forall p q, priq p -> priq q -> priq (merge p q).
@@ -214,9 +292,137 @@ Proof.
 Qed.
 
 (** **** Exercise: 5 stars, standard, optional (delete_max_Some_priq) *)
+(* We restate unzip in a slower but prove-friendly way *)
+Fixpoint unzip'_select n t :=
+  match (n, t) with
+  | (_, Leaf) => Leaf
+  | (O, Node k t1 t2) => Node k t1 Leaf
+  | (S n', Node k t1 t2) => unzip'_select n' t2
+  end.
+
+Fixpoint unzip' n t :=
+  match n with
+  | O => [unzip'_select 0 t]
+  | S n' => unzip'_select n t :: unzip' n' t
+  end.
+
+Eval compute in unzip (Node 4 (Node 3 (Node 1 Leaf Leaf) (Node 1 Leaf Leaf))
+             (Node 3 (Node 2 Leaf Leaf) (Node 5 Leaf Leaf))) (fun _ => nil).
+
+
+Eval compute in unzip' 2 (Node 4 (Node 3 (Node 1 Leaf Leaf) (Node 1 Leaf Leaf))
+             (Node 3 (Node 2 Leaf Leaf) (Node 5 Leaf Leaf))).
+
+Theorem unzip'_select_heap : forall t n1 n2 k,
+  pow2heap' (1 + n1 + n2) k t -> pow2heap n1 (unzip'_select n2 t).
+Proof.
+  intros. generalize dependent t. generalize dependent n1.
+  induction n2; intros; simpl; destruct t; simpl in H; auto.
+  - destruct H as [_ [? _]].
+    rewrite plus_n_O with n1. auto.
+  - apply IHn2. destruct H as [_ [_ ?]].
+    replace (1 + n1 + n2) with (n1 + S n2) by lia. auto.
+Qed.
+
+Theorem unzip'_priq : forall t n1 n2 k,
+  pow2heap' (1 + n1 + n2) k t -> priq' n1 (unzip' n2 t).
+Proof.
+  intros.
+  generalize dependent t.
+  generalize dependent n1.
+  induction n2; intros.
+  - destruct t.
+    + simpl. split; auto.
+      right. simpl in H. destruct H as [_ [? _]].
+      rewrite plus_n_O with n1. auto.
+    + simpl. auto.
+  - simpl; split.
+    + destruct t; auto.
+      right. apply unzip'_select_heap with k.
+      simpl in H. destruct H as [_ [_ ?]].
+      replace (1 + n1 + n2) with (n1 + S n2) by lia. auto.
+    + apply IHn2. replace (1 + S n1 + n2) with (1 + n1 + S n2) by lia.
+      auto.
+Qed.
+
+(* The correctness of unzip' *)
+Theorem unzip'_tail : forall n k t1 t2,
+  unzip' (S n) (Node k t1 t2) = unzip' n t2 ++ [Node k t1 Leaf].
+Proof.
+  induction n; intros.
+  - simpl. auto.
+  - simpl. rewrite <-IHn.
+    simpl. auto.
+Qed.
+
+Theorem unzip'_relate : forall t n k cont,
+  pow2heap' (S n) k t -> unzip t cont = unzip' n t ++ cont [].
+Proof.
+  induction t; intros.
+  - destruct H as [? [? ?]].
+    simpl. destruct n.
+    + simpl in H1. destruct t2; inv H1.
+      simpl. auto.
+    + simpl. rewrite (IHt2 _ _ _ H1).
+      replace (unzip' n t2 ++ Node k t1 Leaf :: cont []) with
+              ((unzip' n t2 ++ [Node k t1 Leaf]) ++ cont [])
+        by (simpl; rewrite <-app_assoc; auto).
+      rewrite <-unzip'_tail. simpl. auto.
+  - simpl in H. destruct H.
+Qed.
+
+Theorem heap_delete_max_priq : forall t n,
+  pow2heap n t ->
+  priq' 0 (heap_delete_max t).
+Proof.
+  intros.
+  destruct t; [|inv H].
+  simpl in *.
+  destruct t2; [inv H|].
+  destruct n.
+  * simpl in H. destruct t1; inv H.
+    simpl. auto.
+  * rewrite (unzip'_relate _ _ _ _ H).
+    rewrite app_nil_r.
+    apply unzip'_priq with k. auto.
+Qed.
+
+Theorem delete_max_aux_priq : forall p p0 p1 n k,
+  priq' n p ->
+  delete_max_aux k p = (p0, p1) ->
+  priq' n p0 /\ priq' 0 p1.
+Proof.
+  induction p; simpl; intros.
+  - inv H0. subst. auto.
+  - destruct a.
+    + destruct a2.
+      * inv H0. subst. split; simpl; auto.
+      * destruct H. destruct H; [inv H|].
+        destruct (k >? k0).
+        -- destruct (delete_max_aux k p) eqn:E.
+           inv H0.
+           destruct (IHp _ _ _ _ H1 E).
+           repeat split; auto.
+        -- inv H0. split.
+           ++ split; auto.
+           ++ exact (heap_delete_max_priq _ _ H).
+    + destruct (delete_max_aux k p) eqn:E.
+      destruct H.
+      inv H0. destruct (IHp _ _ _ _ H1 E).
+      repeat split; auto.
+Qed.
+
 Theorem delete_max_Some_priq:
       forall p q k, priq p -> delete_max p = Some(k,q) -> priq q.
-(* FILL IN HERE *) Admitted.
+Proof.
+  intros.
+  unfold delete_max in H0.
+  destruct (find_max p); inv H0.
+  destruct (delete_max_aux k0 p) eqn:?H. inv H2.
+  destruct (delete_max_aux_priq _ _ _ _ _ H H0).
+  apply join_valid; auto.
+Qed.
+  
 (** [] *)
 
 (* ================================================================= *)
@@ -245,8 +451,12 @@ Inductive tree_elems: tree -> list key -> Prop :=
 *)
 
 Inductive priqueue_elems: list tree -> list key -> Prop :=
-             (* FILL IN HERE *)
-.
+| priqueue_elems_nil: priqueue_elems [] []
+| priqueue_elems_app: forall t l bh bt b,
+    tree_elems t bh ->
+    priqueue_elems l bt ->
+    Permutation b (bh ++ bt) ->
+    priqueue_elems (t :: l) b.
 (* Do not modify the following line: *)
 Definition manual_grade_for_priqueue_elems : option (nat*string) := None.
 (** [] *)
@@ -262,13 +472,33 @@ Definition Abs (p: priqueue) (al: list key) := priqueue_elems p al.
 
 Theorem tree_elems_ext: forall t e1 e2,
   Permutation e1 e2 -> tree_elems t e1 -> tree_elems t e2.
-(* FILL IN HERE *) Admitted.
+Proof.
+  intros. destruct H0.
+  - apply Permutation_nil in H. subst. constructor.
+  - econstructor; [exact H0_|exact H0_0|].
+    eapply perm_trans.
+    + apply Permutation_sym. exact H.
+    + exact H0.
+Qed.
 (** [] *)
 
 (** **** Exercise: 2 stars, standard (tree_perm) *)
 Theorem tree_perm: forall t e1 e2,
   tree_elems t e1 -> tree_elems t e2 -> Permutation e1 e2.
-(* FILL IN HERE *) Admitted.
+Proof.
+  intros.
+  generalize dependent e2.
+  induction H; intros.
+  - inv H0. auto.
+  - inv H2.
+    pose proof (IHtree_elems1 _ H6).
+    pose proof (IHtree_elems2 _ H8).
+    eapply perm_trans.
+    + exact H1.
+    + apply Permutation_sym in H9. eapply perm_trans; [|apply H9].
+      apply perm_skip. apply Permutation_app; auto.
+Qed.
+
 (** [] *)
 
 (** **** Exercise: 2 stars, standard (priqueue_elems_ext)
@@ -278,24 +508,50 @@ Theorem tree_perm: forall t e1 e2,
 
 Theorem priqueue_elems_ext: forall q e1 e2,
   Permutation e1 e2 -> priqueue_elems q e1 -> priqueue_elems q e2.
-(* FILL IN HERE *) Admitted.
+Proof.
+  intros. destruct H0.
+  - apply Permutation_nil in H. subst. constructor.
+  - econstructor; [exact H0 | exact H1 |].
+    eapply perm_trans. { apply Permutation_sym. exact H. }
+    exact H2.
+Qed.
 (** [] *)
 
 (** **** Exercise: 2 stars, standard (abs_perm) *)
+Theorem abs_perm_general: forall p al bl,
+   Abs p al -> Abs p bl -> Permutation al bl.
+Proof.
+  induction p; intros.
+  - inv H. inv H0. auto.
+  - inv H. inv H0.
+    pose proof (tree_perm _ _ _ H3 H2).
+    pose proof (IHp _ _ H4 H5).
+    eapply perm_trans. exact H6.
+    eapply perm_trans. apply Permutation_app; eassumption.
+    apply Permutation_sym. auto.
+Qed.
+
 Theorem abs_perm: forall p al bl,
    priq p -> Abs p al -> Abs p bl -> Permutation al bl.
-Proof.
-(* FILL IN HERE *) Admitted.
-(** [] *)
+Proof. intros. eauto using abs_perm_general. Qed.
 
 (** **** Exercise: 2 stars, standard (can_relate) *)
 Lemma tree_can_relate: forall t, exists al, tree_elems t al.
 Proof.
-(* FILL IN HERE *) Admitted.
+  induction t.
+  - destruct IHt1, IHt2.
+    exists (k :: x ++ x0).
+    econstructor; eauto.
+  - exists []. constructor.
+Qed.
 
 Theorem can_relate:  forall p, priq p -> exists al, Abs p al.
 Proof.
-(* FILL IN HERE *) Admitted.
+  intros. clear H. induction p.
+  - exists []. constructor.
+  - destruct IHp. destruct (tree_can_relate a).
+    exists (x0 ++ x). econstructor; eauto.
+Qed.
 (** [] *)
 
 (* ================================================================= *)
@@ -303,7 +559,8 @@ Proof.
 (** **** Exercise: 1 star, standard (empty_relate) *)
 Theorem empty_relate:  Abs empty nil.
 Proof.
-(* FILL IN HERE *) Admitted.
+  constructor.
+Qed.
 (** [] *)
 
 (** **** Exercise: 3 stars, standard (smash_elems)
@@ -314,7 +571,29 @@ Theorem smash_elems: forall n t u bt bu,
                      pow2heap n t -> pow2heap n u ->
                      tree_elems t bt -> tree_elems u bu ->
                      tree_elems (smash t u) (bt ++ bu).
-(* FILL IN HERE *) Admitted.
+Proof.
+  intros.
+  destruct t; [|inv H].
+  destruct u; [|inv H0].
+  simpl in *.
+  destruct t2; [inv H|]. clear H.
+  destruct u2; [inv H0|]. clear H0.
+  inv H1. inv H6. rewrite app_nil_r in H7.
+  inv H2. inv H6. rewrite app_nil_r in H8.
+  rename k into a. rename k0 into b.
+  rename bl into l1. rename bl0 into l2.
+  bdestruct (a >? b); econstructor; try econstructor; eauto; try constructor;
+    rewrite app_nil_r; eapply perm_trans;
+    try apply Permutation_app; try apply H7; try apply H8; simpl.
+  - (* Permutation (a :: l1 ++ b :: l2) (a :: b :: l2 ++ l1) *)
+    apply perm_skip.
+    apply Permutation_app_comm.
+  - (* Permutation (a :: l1 ++ b :: l2) (b :: a :: l1 ++ l2) *)
+    eapply perm_trans; [|apply perm_swap].
+    apply perm_skip.
+    eapply perm_trans; [apply Permutation_app_comm|].
+    simpl. apply perm_skip. apply Permutation_app_comm.
+Qed.
 (** [] *)
 
 (* ================================================================= *)
@@ -329,14 +608,56 @@ Theorem carry_elems:
       forall eq et, priqueue_elems q eq ->
                           tree_elems t et ->
                           priqueue_elems (carry q t) (eq++et).
-(* FILL IN HERE *) Admitted.
+Proof.
+  intros n q. revert n.
+  induction q; intros.
+  - inv H1. simpl. destruct t.
+    + econstructor; eauto; try econstructor.
+      * apply Permutation_refl. * rewrite app_nil_r. apply Permutation_refl.
+    + inv H2. constructor.
+  - simpl.
+    inv H1.
+    destruct a.
+    + destruct t.
+      * destruct H0; [inv H0|].
+        destruct H. destruct H; [inv H|].
+        econstructor; [constructor | eauto using smash_valid, smash_elems | simpl].
+        eapply perm_trans.
+        -- apply Permutation_app_tail. exact H8.
+        -- rewrite <-app_assoc. apply Permutation_app_rot.
+      * inv H2. rewrite app_nil_r. econstructor; eassumption.
+    + inv H5. simpl in H8.
+      econstructor; try eassumption.
+      eapply perm_trans. apply Permutation_app_comm.
+      apply Permutation_app_head. auto.
+Qed.
 (** [] *)
 
 (** **** Exercise: 2 stars, standard, optional (insert_elems) *)
 Theorem insert_relate:
         forall p al k, priq p -> Abs p al -> Abs (insert k p) (k::al).
-(* FILL IN HERE *) Admitted.
+Proof.
+  intros.
+  eapply priqueue_elems_ext.
+  - apply Permutation_sym.
+    apply Permutation_cons_append.
+  - eapply carry_elems; eauto.
+    + right. constructor.
+    + econstructor; constructor. auto.
+Qed.
 (** [] *)
+
+Lemma Permutation_13_24 : forall pa pb p1 p2 p3 p4 : list key,
+  Permutation pa (p1 ++ p2) ->
+  Permutation pb (p3 ++ p4) ->
+  Permutation (pa ++ pb) (p1 ++ p3 ++ p2 ++ p4).
+Proof.
+  intros.
+  eapply perm_trans. apply Permutation_app; eassumption.
+  repeat rewrite <-app_assoc.
+  apply Permutation_app_head.
+  apply Permutation_app_swap_app.
+Qed.
 
 (** **** Exercise: 4 stars, standard, optional (join_elems) *)
 Theorem join_elems:
@@ -349,7 +670,59 @@ Theorem join_elems:
                              priqueue_elems q qe ->
                              tree_elems c ce ->
                               priqueue_elems (join p q c) (ce++pe++qe).
-(* FILL IN HERE *) Admitted.
+Proof.
+  induction p; intros.
+  - simpl. inv H2. simpl.
+    eapply priqueue_elems_ext. apply Permutation_app_comm.
+    eapply carry_elems; eauto.
+  - inv H2. simpl. destruct a, q.
+    3: { inv H3. rewrite app_nil_r. inv H7. simpl in H10.
+      econstructor; eauto. apply Permutation_app_head. auto. }
+    + destruct H. destruct H; [inv H|]. inv H3. rewrite app_nil_r.
+      destruct c.
+      * destruct H1; [inv H1|].
+        econstructor. constructor.
+        eapply carry_elems; eauto using smash_valid, smash_elems.
+        simpl. eapply perm_trans. apply Permutation_app_head. exact H10.
+        rewrite app_assoc. apply Permutation_app_comm.
+      * inv H4. econstructor; eauto.
+    + inv H. destruct H2; [inv H|].
+      inv H3.
+      destruct t.
+      * inv H0. destruct H2; [inv H0|].
+        econstructor. exact H4.
+        eapply IHp; eauto using smash_valid, smash_elems.
+        apply Permutation_app_head. rewrite <-app_assoc.
+        apply Permutation_13_24; auto.
+      * inv H0. destruct c.
+        -- destruct H1; [inv H0|].
+           econstructor. constructor.
+           eapply IHp; eauto using smash_valid, smash_elems. simpl.
+           rewrite <-app_assoc. apply Permutation_app_head.
+           inv H9. simpl in H13.
+           rewrite app_assoc. apply Permutation_app; auto.
+        -- inv H4. econstructor. eauto.
+           eapply IHp; eauto using smash_valid, smash_elems. simpl.
+           apply Permutation_13_24; auto.
+    + inv H. inv H0. inv H3.
+      destruct t.
+      * inv H; [inv H0|].
+        destruct c.
+        -- inv H1; [inv H|].
+           econstructor. constructor.
+           eapply IHp; eauto using smash_valid, smash_elems.
+           simpl. rewrite <-app_assoc. apply Permutation_app_head. inv H7. simpl in H10.
+           eapply perm_trans. apply Permutation_app; eassumption. apply Permutation_app_swap_app.
+        -- inv H7. simpl in H10. econstructor. eassumption.
+           eapply IHp; eauto using smash_valid, smash_elems.
+           eapply perm_trans; [| apply Permutation_app_swap_app].
+           apply Permutation_app_head. eapply perm_trans; [| apply Permutation_app_swap_app].
+           apply Permutation_app; auto.
+      * inv H11. simpl in H14. econstructor. eassumption.
+        eapply IHp; eauto using smash_valid, smash_elems.
+        apply Permutation_app_head. rewrite app_assoc. apply Permutation_app; auto.
+Qed.
+
 (** [] *)
 
 (** **** Exercise: 2 stars, standard, optional (merge_relate) *)
@@ -359,23 +732,264 @@ Theorem merge_relate:
        Abs p pl -> Abs q ql -> Abs (merge p q) al ->
        Permutation al (pl++ql).
 Proof.
-(* FILL IN HERE *) Admitted.
+  intros.
+  eapply abs_perm.
+  2 : exact H3.
+  - apply merge_priq; auto.
+  - replace (pl ++ ql) with ([] ++ pl ++ ql) by auto.
+    eapply join_elems; eauto. constructor.
+Qed.
 (** [] *)
+
+Theorem find_max_None_relate : forall p,
+  Abs p nil <-> find_max p = None.
+Proof.
+  intros.
+  induction p. { split; auto. constructor. }
+  split; intros.
+  - inv H. apply Permutation_nil in H5. destruct (app_eq_nil _ _ H5). subst.
+    intuition. simpl.
+    destruct a; auto.
+    inv H2. destruct (Permutation_nil_cons H10).
+  - inv H. destruct a; inv H1.
+    intuition.
+    econstructor. constructor. eassumption. auto.
+Qed.
 
 (** **** Exercise: 5 stars, standard, optional (delete_max_None_relate) *)
 Theorem delete_max_None_relate:
         forall p, priq p -> (Abs p nil <-> delete_max p = None).
-(* FILL IN HERE *) Admitted.
+Proof.
+  intros. destruct (find_max_None_relate p).
+  split; intros; intuition.
+  - unfold delete_max. rewrite H3; auto.
+  - apply H1. unfold delete_max in H2. destruct (find_max p); auto.
+    destruct (delete_max_aux k p). inv H2.
+Qed.
 (** [] *)
 
 (** **** Exercise: 5 stars, standard, optional (delete_max_Some_relate) *)
+Theorem tree_ge : forall k l r n tl,
+  pow2heap n (Node k l r) ->
+  tree_elems (Node k l r) tl ->
+  Forall (ge k) tl.
+Proof.
+  intros.
+  simpl in H. destruct r. inv H.
+  inv H0. inv H6. rewrite app_nil_r in H7.
+  eapply Forall_perm. apply Permutation_sym. exact H7. clear H7. clear tl.
+  constructor; auto.
+  revert H H4. revert k n bl.
+  induction l; intros.
+  - destruct n; simpl in H. inv H.
+    destruct H as [? [? ?]].
+    inv H4. eapply Forall_perm. apply Permutation_sym. apply H9.
+    constructor; auto.
+    apply Forall_app. split; eauto.
+    apply Forall_impl with (ge k); eauto. lia.
+  - inv H4. auto.
+Qed.
+
+Theorem find_max'_ge : forall p k,
+  find_max' k p >= k.
+Proof.
+  induction p; intros.
+  - simpl. auto.
+  - simpl. destruct a.
+    + bdestruct (k0 >? k).
+      * specialize IHp with k0. lia.
+      * specialize IHp with k. lia.
+    + specialize IHp with k. lia.
+Qed.    
+
+Theorem priqueue_elems_ge : forall p pl n k0 k,
+  priq' n p ->
+  find_max' k0 p = k ->
+  priqueue_elems p pl ->
+  Forall (ge k) pl.
+Proof.
+  induction p; intros.
+  - inv H1. auto.
+  - inv H. inv H1.
+    destruct a.
+    + destruct H2. inv H.
+      simpl. remember (if k >? k0 then k else k0) as kmax.
+      remember (find_max' kmax p) as k1. symmetry in Heqk1.
+      eapply Forall_perm. apply Permutation_sym, H7.
+      apply Forall_app. split; eauto.
+      pose proof (find_max'_ge p kmax).
+      eapply Forall_impl with (ge k). {
+        intros. bdestruct (k >? k0); lia.
+      }
+      eapply tree_ge; eauto.
+    + inv H4. simpl in H7.
+      simpl. eapply IHp; eauto.
+      eapply priqueue_elems_ext. apply Permutation_sym. eauto. auto.
+Qed.
+
+Theorem unzip_cont_perm : forall t tl pl cont cl,
+  tree_elems t tl ->
+  Abs (cont nil) cl ->
+  Abs (unzip t cont) pl ->
+  Permutation (tl ++ cl) pl.
+Proof.
+  induction t; intros.
+  - simpl in H1.
+    inv H.
+    epose proof (IHt2 _ _ _ (k :: bl ++ cl) H7 _ H1).
+    eapply perm_trans; [| apply H].
+    eapply perm_trans. apply Permutation_app_tail. apply H8.
+    rewrite app_comm_cons.
+    rewrite <-app_assoc. apply Permutation_app_swap_app.
+    Unshelve.
+    simpl. econstructor; eauto.
+    econstructor. exact H5. constructor. rewrite app_nil_r.
+    all: eauto.
+  - simpl in H1. inv H. simpl. eapply abs_perm_general; eauto.
+Qed.
+
+Theorem unzip_perm : forall t tl pl,
+  tree_elems t tl ->
+  Abs (unzip t (fun u => u)) pl ->
+  Permutation tl pl.
+Proof.
+  intros. replace (tl) with (tl ++ []) by apply app_nil_r.
+  eapply unzip_cont_perm; try eassumption.
+  simpl. constructor.
+Qed.
+
+Lemma find_max'_shadow : forall p k k0 k1,
+  find_max' k0 p = k ->
+  k > k0 ->
+  k0 >= k1 ->
+  find_max' k1 p = k.
+Proof.
+  induction p; intros.
+  - simpl in H. try lia.
+  - simpl in *. destruct a.
+    + bdestruct (k2 >? k1); bdestruct (k2 >? k0); try lia;
+      apply IHp with k0; auto.
+    + eapply IHp; eauto.
+Qed.
+
+Theorem find_max_some : forall p k k0,
+  find_max' k0 p = k ->
+  k > k0 ->
+  find_max p = Some k.
+Proof.
+  induction p; intros.
+  - simpl in H. lia.
+  - simpl in *. destruct a.
+    + f_equal. bdestruct (k1 >? k0); auto.
+      eapply find_max'_shadow; eauto.
+    + eauto.
+Qed.
+
+Theorem delete_max_aux_relate : forall p q r pl ql rl k n,
+  priq' n p ->
+  Abs p pl ->
+  find_max p = Some k ->
+  delete_max_aux k p = (q, r) ->
+  Abs q ql ->
+  Abs r rl ->
+  Permutation pl (k :: ql ++ rl) /\ Forall (ge k) pl. (* save your life *)
+Proof.
+  induction p; intros; simpl in *. { inv H1. }
+  destruct H. destruct a.
+  - destruct H. inv H.
+    destruct a2. simpl in H. inv H.
+    bdestruct (k >? k0).
+    + injection H1 as H1.
+      pose proof (find_max_some _ _ _ H1 H6). 
+      destruct (delete_max_aux k p) eqn:E.
+      injection H2 as ?. subst q r.
+      inversion H0. clear H0. subst t l b.
+      pose proof (tree_ge _ _ _ _ _ H H9) as Hbh.
+      inversion H3. clear H3. subst t l b.
+      destruct (IHp _ _ _ _ _ _ _ H5 H10 H7 E H11 H4).
+      clear H1. inv H9. inv H17. rewrite app_nil_r in H18.
+      inv H8. inv H17. rewrite app_nil_r in H19.
+      pose proof (tree_perm _ _ _ H13 H15).
+      split.
+      * (* boring permutation proof *)
+        clear -H14 H19 H12 H18 H0 H1.
+        eapply perm_trans. exact H12.
+        eapply perm_trans. apply Permutation_app. exact H18.
+          exact H0.
+        rewrite app_comm_cons.
+        eapply perm_trans. apply Permutation_app_swap_app .
+        simpl. apply perm_skip.
+        rewrite app_comm_cons. rewrite app_assoc. apply Permutation_app_tail.
+        eapply perm_trans. 2: apply Permutation_sym; exact H14.
+        eapply perm_trans. apply Permutation_app_comm. apply Permutation_app_tail.
+        apply Permutation_sym. eapply perm_trans. exact H19. apply perm_skip. auto.
+      * eapply Forall_perm. apply Permutation_sym. exact H12.
+        apply Forall_app. split; auto.
+        apply Forall_impl with (ge k0). lia. auto.
+    + inv H2. inv H3. inv H8. simpl in H11. inv H0.
+      pose proof (tree_ge _ _ _ _ _ H H7).
+      inv H7. inv H15. rewrite app_nil_r in H16.
+      Check unzip_perm.
+      pose proof (unzip_perm _ _ _ H13 H4).
+      injection H1 as H1.
+      Check priqueue_elems_ge.
+      pose proof (priqueue_elems_ge _ _ _ _ _ H5 H1 H8).
+      Check find_max'_ge. pose proof (find_max'_ge p k0).
+      rewrite H1 in H7. clear H1. assert (k0 = k) by lia. subst k0.
+      Check abs_perm_general.
+      pose proof (abs_perm_general _ _ _ H8 H9).
+      split.
+      * clear -H2 H11 H12 H16 H1.
+        eapply perm_trans. apply H12. eapply perm_trans.
+          apply Permutation_app; eassumption.
+        simpl. apply perm_skip. eapply perm_trans. apply Permutation_app_tail. apply H2.
+        eapply perm_trans. apply Permutation_app_comm. apply Permutation_app_tail.
+        apply Permutation_sym. auto.
+      * eapply Forall_perm. apply Permutation_sym. apply H12.
+        apply Forall_app. split; auto.
+  - destruct (delete_max_aux k p) eqn:E.
+    inv H2. inv H3. inv H7. simpl in H10.
+    inv H0. inv H6. simpl in H11.
+    apply Permutation_sym in H11.
+    pose proof (priqueue_elems_ext _ _ _ H11 H7).
+    destruct (IHp _ _ _ _ _ _ _ H5 H0 H1 E H8 H4).
+    split; auto.
+    eapply perm_trans. exact H2. apply perm_skip. apply Permutation_app_tail.
+    apply Permutation_sym. auto.
+Qed.
+
 Theorem delete_max_Some_relate:
   forall (p q: priqueue) k (pl ql: list key), priq p ->
    Abs p pl ->
    delete_max p = Some (k,q) ->
    Abs q ql ->
    Permutation pl (k::ql) /\ Forall (ge k) ql.
-(* FILL IN HERE *) Admitted.
+Proof.
+  intros.
+  unfold delete_max in H1.
+  destruct (find_max p) eqn:E; [| inv H1].
+  destruct (delete_max_aux k0 p) eqn:?E.
+  inv H1.
+  Check delete_max_aux_priq.
+  destruct (delete_max_aux_priq _ _ _ _ _ H E0).
+  destruct (can_relate _ H1).
+  destruct (can_relate _ H3).
+  Check join_elems.
+  epose proof (join_elems _ _ Leaf _ H1 H3 _ _ _ nil H4 H5 _).
+  Unshelve. 2: auto. 2: constructor.
+  simpl in H6.
+  Check delete_max_aux_relate.
+  destruct (delete_max_aux_relate _ _ _ _ _ _ _ _ H H0 E E0 H4 H5).
+  Check abs_perm_general.
+  pose proof (abs_perm_general _ _ _ H2 H6).
+  apply Permutation_sym in H9.
+  split.
+  - eapply perm_trans. exact H7. apply perm_skip. auto.
+  - eapply Forall_perm in H8. 2: apply H7.
+    inv H8.
+    eapply Forall_perm. apply H9. auto.
+Qed.
+
 (** [] *)
 
 (** With the following line, we're done!  We have demonstrated that
